Total correctness for existential Hoare logic. Almost finish the proofs.

theories/EHoare.v
@@ -1,4 +1,10 @@
-Require Import Coq.Program.Tactics.
+Require Import
+        Coq.Arith.Arith
+        Coq.micromega.Psatz
+        Coq.Logic.Classical
+        Coq.Logic.ClassicalUniqueChoice
+        Coq.Program.Tactics.
+
 Require Import Maps Imp HoareCommon.
 
 Section EHoare.
@@ -8,7 +14,6 @@ Context {env : Env}.
 Definition ehoare_triple
            (P : Assertion) (c : com) (Q : Assertion) : Prop :=
   forall st,
-     (exists st', st =[ c ]=> st') ->
      P st ->
      exists st', st =[ c ]=> st' /\ Q st'.
 
@@ -17,7 +22,7 @@ Notation "{{ P }}  c  {{ Q }}#" :=
   : hoare_spec_scope.
 
 Definition ewp (c:com) (Q:Assertion) : Assertion :=
-  fun st => (exists st', st =[ c ]=> st') -> exists st', st =[ c ]=> st' /\ Q st'.
+  fun st => exists st', st =[ c ]=> st' /\ Q st'.
 
 Lemma ewp_is_precondition: forall c Q,
   {{ewp c Q}} c {{Q}}#.
@@ -34,12 +39,16 @@ Qed.
 Reserved Notation "|- {{ P }}  c  {{ Q }}#"
          (at level 90, c at next level).
 
-Inductive ehoare_proof : Assertion -> com -> Assertion -> Type :=
+Inductive ehoare_proof : Assertion -> com -> Assertion -> Prop :=
   | EH_Skip : forall P,
       |- {{P}} SKIP {{P}}#
   | EH_Asgn : forall Q V a,
-      |- {{assn_sub V a Q}} V ::= a {{Q}}#
-  (* EH_Spec *)
+      |- {{Q[V |-> a]}} V ::= a {{Q}}#
+  | EH_Spec : forall Q y f xs,
+      |- {{fun st =>
+            (funsig f).(pre) (aseval st xs) /\
+            exists v, (funsig f).(post) v (aseval st xs) /\
+                 Q[y |-> v] st}} y :::= f $ xs {{Q}}#
   | EH_Seq  : forall P c Q d R,
       |- {{P}} c {{Q}}# -> |- {{Q}} d {{R}}# ->
       |- {{P}} c;;d {{R}}#
@@ -47,8 +56,10 @@ Inductive ehoare_proof : Assertion -> com -> Assertion -> Type :=
       |- {{fun st => P st /\ bassn b st}} c1 {{Q}}# ->
       |- {{fun st => P st /\ ~(bassn b st)}} c2 {{Q}}# ->
       |- {{P}} TEST b THEN c1 ELSE c2 FI {{Q}}#
-  | EH_While : forall P b c,
-      |- {{fun st => P st /\ bassn b st}} c {{P}}# ->
+  | EH_While : forall P E b c,
+      (forall n : nat, |- {{fun st => P st /\ bassn b st /\ E st = n}} c {{fun st => P st /\ E st < n}}#) ->
+      (* E st is nat. *)
+      (* (forall st, P st /\ bassn b st -> 0 <= E st) -> *)
       |- {{P}} WHILE b DO c END {{fun st => P st /\ ~ (bassn b st)}}#
   | EH_Consequence  : forall (P Q P' Q' : Assertion) c,
       |- {{P'}} c {{Q'}}# ->
@@ -65,30 +76,188 @@ Hint Constructors ehoare_proof : hoare.
 Hint Unfold ehoare_triple ewp.
 Hint Constructors ceval.
 
+Lemma ehoare_while : forall P E b c,
+    (forall n : nat, {{fun st => P st /\ bassn b st /\ E st = n}} c {{fun st => P st /\ E st < n}}#) ->
+    {{P}} WHILE b DO c END {{fun st => P st /\ ~ (bassn b st)}}#.
+Proof.
+  unfold ehoare_triple.
+  intros. remember (E st). revert dependent st.
+  induction n as [n IH] using (well_founded_ind lt_wf). intros. subst.
+  destruct (beval st b) eqn:?.
+  - edestruct H; eauto. destruct_conjs.
+    edestruct IH; eauto. destruct_conjs.
+    eauto.
+  - firstorder with hoare.
+Qed.
+
 Theorem ehoare_proof_sound : forall P c Q,
     |- {{P}} c {{Q}}# -> {{P}} c {{Q}}#.
 Proof.
   unfold ehoare_triple.
-  intros ? ? ? pf. induction pf; intros st [st' HE] HP.
+  intros ? ? ? pf. induction pf; intros st HP.
   - (* SKIP *)
-    inversion HE; subst. eauto.
+    eauto.
   - (* ::= *)
-    inversion HE; subst. eauto.
+    repeat econstructor. eauto.
+  - (* :::= *)
+    destruct_conjs.
+    repeat econstructor; eauto.
   - (* ;; *)
-    admit.
-  - (* TEST *)
-    inversion HE; subst.
     firstorder eauto.
-    edestruct IHpf2; intuition eauto. congruence.
+  - (* TEST *)
+    destruct (beval st b) eqn:?; firstorder with hoare.
   - (* WHILE *)
-    admit.
+    eapply ehoare_while; eauto.
   - (* Conseq *)
     firstorder eauto.
-Admitted.
+Qed.
+
+Inductive loop_sizeR : forall {st c st'}, st =[ c ]=> st' -> nat -> Prop :=
+| LS_WhileFalse : forall b st c pff,
+    loop_sizeR (E_WhileFalse b st c pff) 0
+| LS_WhileTrue : forall st st' st'' b c pft pfc pfw n,
+    loop_sizeR pfw n ->
+    loop_sizeR (E_WhileTrue st st' st'' b c pft pfc pfw) (S n)
+.
+
+Definition loop_measureR b c (Q : Assertion)
+           (st : state) (n : nat) : Prop :=
+  (~ (exists st', st =[ WHILE b DO c END ]=> st' /\ Q st') -> n = 0) /\
+  (forall m st' (pf : st =[ WHILE b DO c END ]=> st'),
+      Q st' ->
+      loop_sizeR pf m ->
+      (forall m' st'' (pf' : st =[ WHILE b DO c END ]=> st''),
+          Q st'' ->
+          loop_sizeR pf' m' ->
+          m <= m') ->
+      n = m).
+
+Scheme ceval_ind_dep := Induction for ceval Sort Prop.
+
+Lemma loop_sizeR_ex : forall st b c st' (pf : st =[ WHILE b DO c END ]=> st'),
+    exists n, loop_sizeR pf n.
+Proof.
+  intros. remember (WHILE b DO c END)%imp as c' eqn:Heq.
+  induction pf using ceval_ind_dep; inversion Heq; subst.
+  - repeat econstructor.
+  - destruct IHpf2; auto. repeat econstructor. eauto.
+Qed.
+
+Lemma loop_sizeR_inv : forall st st' st'' b c pft pfc pfw n,
+    loop_sizeR (E_WhileTrue st st' st'' b c pft pfc pfw) n ->
+    exists m, loop_sizeR pfw m /\ S m = n.
+Proof.
+  Admitted.
+
+Lemma nonempty_smallest_ex (P : nat -> Prop) :
+  (exists n, P n) ->
+  exists n, P n /\ (forall n', P n' -> n <= n').
+Proof.
+  intros [n H]. induction n using (well_founded_ind lt_wf).
+  destruct (classic (exists y, y < n /\ P y)).
+  - firstorder.
+  - exists n. intuition. apply Nat.nlt_ge. eauto.
+Qed.
+
+Lemma loop_measureR_ex b c Q st :
+  (exists st', st =[ WHILE b DO c END ]=> st' /\ Q st') ->
+  exists m st' (pf : st =[ WHILE b DO c END ]=> st'),
+    Q st' /\ loop_sizeR pf m /\
+    (forall m' st'' (pf' : st =[ WHILE b DO c END ]=> st''),
+        Q st'' -> loop_sizeR pf' m' -> m <= m').
+Proof.
+  intros.
+  edestruct (nonempty_smallest_ex
+               (fun m => exists st' (pf : st =[ WHILE b DO c END ]=> st'),
+                    Q st' /\ loop_sizeR pf m)) as [m ?].
+  - destruct H as [? [H ?]]. edestruct loop_sizeR_ex with (pf:=H). eauto.
+  - destruct_conjs. exists m. repeat econstructor; eauto.
+Qed.
+
+Lemma loop_measureR_is_fun b c Q : forall (st : state),
+    exists! n, loop_measureR b c Q st n.
+Proof.
+  unfold unique.
+  intros. destruct (classic (exists st', st =[ WHILE b DO c END ]=> st' /\ Q st')) as [H | H].
+  - apply loop_measureR_ex in H. destruct H as [m [st' [pf ?]]]. destruct_conjs.
+    exists m. split.
+    + split. intros. exfalso. eauto.
+      intros m'. intros. assert (m <= m') by eauto. assert (m' <= m) by eauto.
+      lia.
+    + intros ? H'. destruct H' as [? H'].
+      symmetry. eauto.
+  - exists 0. split.
+    + split; intros; eauto. exfalso. eauto.
+    + intros ? H'. destruct H' as [? H'].
+      symmetry. eauto.
+Qed.
+
+Lemma loop_measureR_order : forall (Q : Assertion) st st' st'' b c pft pfc pfw m,
+    Q st'' ->
+    loop_sizeR (E_WhileTrue st st' st'' b c pft pfc pfw) m ->
+    (forall m' st''' (pf' : st =[ WHILE b DO c END ]=> st'''),
+        Q st''' ->
+        loop_sizeR pf' m' ->
+        m <= m') ->
+    forall m', loop_measureR b c Q st' m' ->
+          S m' = m.
+Proof.
+  intros until m. intros HQ Hs H m' H'. destruct H' as [_ H'].
+  apply loop_sizeR_inv in Hs. destruct Hs as [n [? ?]].
+  subst. f_equal. eapply H'; eauto.
+  intros. apply le_S_n.
+  eapply H; eauto. constructor. eauto.
+  Grab Existential Variables.
+  all : eauto.
+Qed.
 
 Theorem ehoare_proof_complete: forall P c Q,
     {{P}} c {{Q}}# -> |- {{P}} c {{Q}}#.
 Proof.
-  Admitted.
+  unfold ehoare_triple.
+  intros P c. revert dependent P.
+  induction c; intros P Q HT.
+  - (* SKIP *)
+    eapply EH_Consequence; eauto with hoare.
+    intros. edestruct HT as [? [HE ?]]; eauto.
+    inversion HE; subst. eauto.
+  - (* ::= *)
+    eapply EH_Consequence; eauto with hoare.
+    intros. edestruct HT as [? [HE ?]]; eauto.
+    inversion HE; subst. eauto.
+  - (* :::= *)
+    eapply EH_Consequence; eauto with hoare.
+    simpl. intros. edestruct HT as [? [HE ?]]; eauto.
+    inversion HE; subst. eauto.
+  - (* ;; *)
+    apply EH_Seq with (ewp c2 Q); eauto. apply IHc1.
+    intros. edestruct HT as [? [HE ?]]; eauto.
+    inversion HE; subst. firstorder.
+  - (* IFB *)
+    apply EH_If.
+    + apply IHc1. intros. destruct_conjs.
+      edestruct HT as [? [HE ?]]; eauto.
+      inversion HE; subst; firstorder with hoare.
+    + apply IHc2. intros. destruct_conjs.
+      edestruct HT as [? [HE ?]]; eauto.
+      inversion HE; subst; firstorder with hoare.
+  - (* WHILE *)
+    eapply EH_Consequence with (P':=ewp (WHILE b DO c END) Q).
+    + destruct (unique_choice _ _
+                              (loop_measureR b c Q)
+                              (loop_measureR_is_fun b c Q)) as [measure Hm].
+      apply EH_While with (E:=measure).
+      intros. apply IHc. intros ? [Hwp ?]. destruct_conjs. subst.
+      destruct (Hm st) as [_ Hm'].
+      edestruct loop_measureR_ex as [m [st' [pf ?]]]; eauto. destruct_conjs.
+      remember (WHILE b DO c END)%imp eqn:Heq.
+      destruct pf; inversion Heq; subst; clear Heq. exfalso. congruence.
+      eexists. intuition eauto.
+      eapply loop_measureR_order in Hm; eauto.
+      assert (measure st = m) by eauto. lia.
+    + eauto.
+    + simpl. intros ? [H ?]. destruct H as [? [H ?]].
+      inversion H; subst; eauto. exfalso. eauto.
+Qed.
 
 End EHoare.
